format-version: 1.2
date: 03:05:2017 16:19
saved-by: jesmith
auto-generated-by: OBO-Edit 2.3.1
default-namespace: chinchilla_species_and_sources

[Term]
id: CS:0000000
name: Chinchilla species and sources
created_by: JSmith
creation_date: 2015-04-21T14:10:45Z

[Term]
id: CS:0000001
name: Chinchilla lanigera
def: "The chinchilla species with common name long-tailed chinchilla." [Taxon:34839]
synonym: "long-tailed chinchilla" RELATED []
xref: NCBI_Taxon:34839
is_a: CS:0000000 ! Chinchilla species and sources
created_by: JSmith
creation_date: 2015-04-21T14:11:27Z

[Term]
id: CS:0000002
name: Rrcjo:Chin
def: "Outbred animals of species Chinchilla laniger sourced from R&R Chinchilla, Jenera, OH." [PMID:20591507, RGD:JRS]
is_a: CS:0000001 ! Chinchilla lanigera
created_by: JSmith
creation_date: 2015-04-21T14:17:09Z

[Term]
id: CS:0000003
name: Unsps:Chin
def: "Outbred animals of species Chinchilla laniger from an unspecified source." [RGD:JRS]
is_a: CS:0000001 ! Chinchilla lanigera
created_by: JSmith
creation_date: 2015-04-21T14:28:50Z

[Term]
id: CS:0000004
name: Raulo:Chin
def: "Outbred animals of species Chinchilla laniger sourced from Rauscher's chinchilla ranch, Larue, OH." [PMID:23092856, PMID:25348637, RGD:JRS]
is_a: CS:0000001 ! Chinchilla lanigera
created_by: JSmith
creation_date: 2015-04-21T14:32:29Z

[Term]
id: CS:0000005
name: Ryepo:Chin
def: "Outbred animals of species Chinchilla laniger sourced from Ryerson Chinchilla Ranch, Plymouth, OH." [PMID:25734113, RGD:JRS]
is_a: CS:0000001 ! Chinchilla lanigera
created_by: JSmith
creation_date: 2015-04-21T17:39:46Z

[Term]
id: CS:0000006
name: Ritjo:Chin
def: "Outbred animals of species Chinchilla laniger sourced from Ritterspach Chinchilla Ranch, Jenera, OH." [RGD:JRS]
is_a: CS:0000001 ! Chinchilla lanigera
created_by: JSmith
creation_date: 2015-04-22T11:03:20Z

[Term]
id: CS:0000007
name: Mccnwp:Chin
def: "Outbred animals of species Chinchilla laniger sourced from McClenahan Chinchilla Ranch, New Wilmington, PA." [PMID:20433028, RGD:JRS]
is_a: CS:0000001 ! Chinchilla lanigera
created_by: JSmith
creation_date: 2015-04-22T11:49:32Z

[Term]
id: CS:0000008
name: Mourm:Chin
def: "Outbred animals of species Chinchilla laniger sourced from Moulton Chinchilla Ranch, Rochester, MN." [PMID:19782149, RGD:JRS]
is_a: CS:0000001 ! Chinchilla lanigera
created_by: JSmith
creation_date: 2015-04-22T13:16:32Z

[Term]
id: CS:0000009
name: Chinchilla chinchilla
def: "The chinchilla species with the common name short-tailed chinchillas." [NCBI_Taxon:10152]
synonym: "short-tailed chinchilla" RELATED []
xref: NCBI_Taxon:10152
is_a: CS:0000000 ! Chinchilla species and sources
created_by: JSmith
creation_date: 2015-04-22T13:27:18Z

[Term]
id: CS:0000010
name: Bocecw:Chin
def: "Outbred animals of species Chinchilla laniger from Bobbie's Chinchillas in Eau Claire, WI." [RGD:JRS]
synonym: "BS" RELATED []
is_a: CS:0000001 ! Chinchilla lanigera
created_by: jesmith
creation_date: 2017-05-03T12:17:50Z

[Term]
id: CS:0000011
name: Bbcdw:Chin
def: "Outbred animals of species Chinchilla laniger from B and B Chinchillas in Dodgeville, WI." [RGD:JRS]
synonym: "Walt" RELATED []
is_a: CS:0000001 ! Chinchilla lanigera
created_by: jesmith
creation_date: 2017-05-03T12:19:07Z

[Term]
id: CS:0000012
name: Abcci:Chin
def: "Outbred animals of species Chinchilla laniger from ABC Chinchillas in Cary, IL." [RGD:JRS]
synonym: "Mor" RELATED []
is_a: CS:0000001 ! Chinchilla lanigera
created_by: jesmith
creation_date: 2017-05-03T12:21:07Z

[Term]
id: CS:0000013
name: Wkdmw:Chin
def: "Outbred animals of species Chinchilla laniger from WK's Designer Chins in Mosinee, WI." [RGD:JRS]
synonym: "Torgerson" RELATED []
is_a: CS:0000001 ! Chinchilla lanigera
created_by: jesmith
creation_date: 2017-05-03T12:22:15Z

[Term]
id: CS:0000014
name: Cecww:Chin
def: "Outbred animals of species Chinchilla laniger bred by C. F. in Wautoma, WI." [RGD:JRS]
comment: C. F. is Cecil Featherston.
synonym: "Cecil" RELATED []
is_a: CS:0000001 ! Chinchilla lanigera
created_by: jesmith
creation_date: 2017-05-03T12:23:47Z

